poly 64

snapshots/aes-bslice/aes_bslice4.c
@@ -3,13 +3,14 @@
 #include <string.h> 
 #include <sys/types.h> 
 #include "endianness.h"
+#include "x86intrin.h"
 
 typedef uint64_t* transpose_t;
 
 //#define static static inline __attribute((always_inline))
 
 static uint64_t transpose64(uint64_t x) {
-  uint64_t y = 0;
+ uint64_t y = 0;
 
   y =  (x & 0x8040201008040201LL)        |
     ((x & 0x4020100804020100LL) >>  7) |
@@ -26,7 +27,20 @@ static uint64_t transpose64(uint64_t x) {
     ((x << 35) & 0x0402010000000000LL) |
     ((x << 42) & 0x0201000000000000LL) |
     ((x << 49) & 0x0100000000000000LL);
-  
+  return y;
+}
+
+static uint64_t transpose64_bmi(uint64_t x) {
+ uint64_t y = 0;
+
+ y =  _pext_u64(x,0x0101010101010101) |
+   (_pext_u64(x,0x0202020202020202) << 8) |
+   (_pext_u64(x,0x0404040404040404) << 16) |
+   (_pext_u64(x,0x0808080808080808) << 24) |
+   (_pext_u64(x,0x1010101010101010) << 32) |
+   (_pext_u64(x,0x2020202020202020) << 40) |
+   (_pext_u64(x,0x4040404040404040) << 48) |
+   (_pext_u64(x,0x8080808080808080) << 56);
   return y;
 }
 
@@ -56,11 +70,11 @@ static  void to_transpose_block(transpose_t out, uint8_t* in) {
   }
 }
 
-static void from_transpose(uint8_t* out, transpose_t in) {
-  uint64_t t0 = (in[0] & 0xffffffff) ^ (in[4] << 32);
-  uint64_t t1 = (in[1] & 0xffffffff) ^ (in[5] << 32);
-  uint64_t t2 = (in[2] & 0xffffffff) ^ (in[6] << 32);
-  uint64_t t3 = (in[3] & 0xffffffff) ^ (in[7] << 32);
+static void from_transpose(uint64_t* out, transpose_t in) {
+  uint64_t t0 = (in[4] << 32) ^ (in[0] & 0xffffffff);
+  uint64_t t1 = (in[5] << 32) ^ (in[1] & 0xffffffff);
+  uint64_t t2 = (in[6] << 32) ^ (in[2] & 0xffffffff);
+  uint64_t t3 = (in[7] << 32) ^ (in[3] & 0xffffffff);
 
   
   uint64_t t4 = (in[4] & 0xffffffff00000000) ^ (in[0] >> 32);
@@ -123,14 +137,23 @@ static void from_transpose(uint8_t* out, transpose_t in) {
   t6 = transpose64(t6);
   t7 = transpose64(t7);
 
-  store64_le(out,t0);
+  out[0] = t0;
+  out[1] = t1;
+  out[2] = t2;
+  out[3] = t3;
+  out[4] = t4;
+  out[5] = t5;
+  out[6] = t6;
+  out[7] = t7;
+  
+  /*  store64_le(out,t0);
   store64_le(out+8,t1);
   store64_le(out+16,t2);
   store64_le(out+24,t3);
   store64_le(out+32,t4);
   store64_le(out+40,t5);
   store64_le(out+48,t6);
-  store64_le(out+56,t7);
+  store64_le(out+56,t7); */
 
 }
 
@@ -301,14 +324,14 @@ static  void mixColumns(transpose_t st) {
     rot_prev = col01;
     }*/
   uint64_t col[8] = {0};
-  //#pragma unroll
+  #pragma unroll
   for (int i = 0; i < 8; i++) {
     col[i] = st[i] ^ (((st[i] & 0xeeeeeeeeeeeeeeee) >> 1) | ((st[i] & 0x1111111111111111) << 3));
   }
 
   uint64_t ncol = col[0] ^ (((col[0] & 0xcccccccccccccccc ) >> 2) | ((col[0] & 0x3333333333333333) << 2));
   st[0] = st[0] ^ ncol;
-  //#pragma unroll
+  #pragma unroll
   for (int i = 1; i < 8; i++) {
     uint64_t coli = col[i] ^ (((col[i] & 0xcccccccccccccccc ) >> 2) | ((col[i] & 0x3333333333333333) << 2));
     st[i] = st[i] ^ coli ^ col[i-1];
@@ -334,9 +357,9 @@ static  void addRoundKey(transpose_t st, transpose_t k) {
 }
 
 inline static  void aes_enc(transpose_t st, transpose_t k) {
-  subBytes(st);      // 10-12 cy
-  shiftRows(st);     // 4 cy
-  mixColumns(st);    // 8-10 cy
+  subBytes(st);      // 7-8 cy
+  shiftRows(st);     // 2-3 cy
+  mixColumns(st);    // 5 cy
   addRoundKey(st,k); // 3 cy
 }
 
@@ -357,10 +380,10 @@ static  void rounds(transpose_t st, uint64_t* key) {
   aes_enc(st,key+40);
   aes_enc(st,key+48);
   aes_enc(st,key+56);
-  aes_enc(st,key+64); 
+  aes_enc(st,key+64);  
 }
 
-static void block_cipher(uint8_t* out, uint64_t* st, uint64_t* key) {
+static void block_cipher(uint64_t* out, uint64_t* st, uint64_t* key) {
   uint64_t* k0 = key;
   uint64_t* k = key + 8;
   uint64_t* kn = key + (8 * 10);
@@ -399,7 +422,7 @@ static void key_expansion(uint64_t* out, uint8_t* key) {
     key_expansion_step(out+(8*i),out+(8*i-8),rcon[i]);
 }
 
-static void aes128_block(uint8_t* out, uint64_t* kex, uint64_t* nt, uint32_t c) {
+static void aes128_block(uint64_t* out, uint64_t* kex, uint64_t* nt, uint32_t c) {
   uint8_t ctr[16] = {0};
   for (int i = 0; i < 4; i++) 
     store32_be(ctr+(4*i),c + i);
@@ -424,12 +447,12 @@ static void aes128_ctr(uint8_t* out, uint8_t* in, int in_len, uint8_t* k, uint8_
   uint64_t nt[8] = {0};
   to_transpose_block_copy(nt,nb);
   
-  uint8_t kb[64] = {0};
+  uint64_t kb[8] = {0};
   int blocks64 = in_len / 64;
   for (int i = 0; i < blocks64; i++) {
     aes128_block(kb,kex,nt,c+(4*i));
-    for (int j = 0; j < 64; j++) {
-      out[64*i+j] = in[64*i+j] ^ kb[j];
+    for (int j = 0; j < 8; j++) {
+      store64_le(out+64*i+8*j,load64_le(in+64*i+8*j) ^ kb[j]);
     }
   }
 
@@ -438,10 +461,13 @@ static void aes128_ctr(uint8_t* out, uint8_t* in, int in_len, uint8_t* k, uint8_
     in = in + (64 * blocks64);
     out = out + (64 * blocks64);
     c = c + (4 * blocks64);
+    uint8_t last[64] = {0};
+    memcpy(last,in,rem);
     aes128_block(kb,kex,nt,c);
-    for (int j = 0; j < rem; j++) {
-      out[j] = in[j] ^ kb[j];
+    for (int j = 0; j < 8; j++) {
+      store64_le(last+8*j,load64_le(last+8*j) ^ kb[j]);
     }
+    memcpy(out,last,rem);
   }
 }
 
