code/aes/Hacl.Impl.Poly1305.Fields.fst
@@ -1,0 +1,153 @@
+module Hacl.Impl.Poly1305.Fields
+
+module ST = FStar.HyperStack.ST
+open FStar.HyperStack
+open FStar.HyperStack.All
+open Lib.IntTypes
+open LowStar.Buffer
+open Lib.Utils
+module F64 = Hacl.Impl.Poly1305.Field64
+
+type field_spec = 
+  | M32
+  | M64
+
+
+unfold
+let limb (s:field_spec) =
+  match s with
+  | M32 -> uint32
+  | M64 -> uint64
+
+unfold
+let limb_zero (s:field_spec) : limb s=
+  match s with
+  | M32 -> u32 0 
+  | M64 -> u64 0
+
+unfold
+let wide (s:field_spec) =
+  match s with
+  | M32 -> uint64
+  | M64 -> uint128
+
+unfold
+let nlimb (s:field_spec) : size_nat =
+  match s with
+  | M32 -> 5
+  | M64 -> 3
+
+
+type felem (s:field_spec) = lbuffer (limb s) (nlimb s)
+type felem_wide (s:field_spec) = lbuffer (wide s) (nlimb s)
+
+noextract 
+val as_nat: #s:field_spec -> h:mem -> e:felem s-> GTot nat 
+let as_nat #s h e = 
+  match s with
+  | M32 -> admit()
+  | M64 -> F64.as_nat h e
+  
+inline_for_extraction
+val create_felem: s:field_spec -> StackInline (felem s)
+                   (requires (fun h -> True))
+		   (ensures (fun h0 f h1 -> live h1 f 
+			    /\ as_nat h1 f == 0))
+let create_felem s = 
+  match s with
+  | M32 -> admit()
+  | M64 -> F64.create_felem ()
+
+
+inline_for_extraction
+val carry_felem: #s:field_spec -> f:felem s -> Stack unit
+                   (requires (fun h -> live h f))
+		   (ensures (fun h0 _ h1 -> modifies (loc_buffer f) h0 h1))
+let carry_felem #s f =
+  match s with
+  | M32 -> admit()
+  | M64 -> F64.carry_felem f
+
+inline_for_extraction
+val carry_top_felem: #s:field_spec -> f:felem s -> Stack unit
+                   (requires (fun h -> live h f))
+		   (ensures (fun h0 _ h1 -> modifies (loc_buffer f) h0 h1))
+let carry_top_felem #s f =
+  match s with
+  | M32 -> admit()
+  | M64 -> F64.carry_top_felem f
+
+inline_for_extraction
+val load_felem: #s:field_spec -> f:felem s -> lo:uint64 -> hi:uint64 -> Stack unit
+                   (requires (fun h -> live h f))
+		   (ensures (fun h0 _ h1 -> modifies (loc_buffer f) h0 h1))
+let load_felem (#s:field_spec) (f:felem s) (lo:uint64) (hi:uint64) = 
+  match s with
+  | M32 -> admit()
+  | M64 -> F64.load_felem f lo hi
+
+inline_for_extraction
+val store_felem: #s:field_spec -> f:felem s -> Stack (lo:uint64 * hi:uint64)
+                   (requires (fun h -> live h f))
+		   (ensures (fun h0 _ h1 -> h0 == h1))
+let store_felem (#s:field_spec) (f:felem s) =
+  match s with
+  | M32 -> admit()
+  | M64 -> F64.store_felem f 
+
+inline_for_extraction
+val set_bit: #s:field_spec -> f:felem s -> i:size_t{size_v i < 130} -> Stack unit
+                   (requires (fun h -> live h f))
+		   (ensures (fun h0 _ h1 -> modifies (loc_buffer f) h0 h1))
+let set_bit (#s:field_spec) (f:felem s) (i:size_t{size_v i < 130}) = 
+  match s with
+  | M32 -> admit()
+  | M64 -> F64.set_bit f i
+
+inline_for_extraction
+val set_bit128: #s:field_spec -> f:felem s -> Stack unit
+                   (requires (fun h -> live h f))
+		   (ensures (fun h0 _ h1 -> modifies (loc_buffer f) h0 h1))
+let set_bit128 (#s:field_spec) (f:felem s) = 
+  match s with
+  | M32 -> admit()
+  | M64 -> F64.set_bit128 f
+
+
+inline_for_extraction
+val set_zero: #s:field_spec -> f:felem s -> Stack unit
+                   (requires (fun h -> live h f))
+		   (ensures (fun h0 _ h1 -> modifies (loc_buffer f) h0 h1))
+let set_zero (#s:field_spec) (f:felem s) = 
+  match s with
+  | M32 -> admit()
+  | M64 -> F64.set_zero f
+
+inline_for_extraction
+val smul20_felem: #s:field_spec -> f1:felem s -> f2:felem s-> Stack unit
+                   (requires (fun h -> live h f1 /\ live h f2))
+		   (ensures (fun h0 _ h1 -> modifies (loc_buffer f1) h0 h1))
+let smul20_felem #s f1 f2 = 
+  match s with
+  | M32 -> admit()
+  | M64 -> F64.smul20_felem f1 f2
+
+
+inline_for_extraction
+val fadd_mul_felem: #s:field_spec -> acc:felem s -> f1:felem s -> f2:felem s -> f2_20:felem s -> Stack unit
+                   (requires (fun h -> live h acc /\ live h f1 /\ live h f2 /\ live h f2_20))
+		   (ensures (fun h0 _ h1 -> modifies (loc_buffer acc) h0 h1))
+let fadd_mul_felem #s acc f1 f2 f2_20 =
+  match s with
+  | M32 -> admit()
+  | M64 -> F64.fadd_mul_felem acc f1 f2 f2_20
+
+inline_for_extraction
+val add_felem: #s:field_spec -> f1:felem s -> f2:felem s -> Stack unit
+                   (requires (fun h -> live h f1 /\ live h f2))
+		   (ensures (fun h0 _ h1 -> modifies (loc_buffer f1) h0 h1))
+let add_felem #s f1 f2=
+  match s with
+  | M32 -> admit()
+  | M64 -> admit(); F64.add_felem f1 f2 
+
