code/aes/Hacl.Impl.Poly1305.fst
@@ -1,0 +1,162 @@
+module Hacl.Impl.Poly1305
+
+module ST = FStar.HyperStack.ST
+open FStar.HyperStack
+open FStar.HyperStack.All
+open Lib.IntTypes
+open LowStar.Buffer
+open Lib.Utils
+
+open Hacl.Impl.Poly1305.Fields
+
+inline_for_extraction
+val poly1305_encode_block: #s:field_spec -> f:felem s -> b:lbytes 16 -> Stack unit
+                   (requires (fun h -> live h b /\ live h f ))
+		   (ensures (fun h0 _ h1 -> modifies (loc_buffer f) h0 h1))
+let poly1305_encode_block #s f b = 
+    let (lo,hi) = load64x2_le b in
+    load_felem f lo hi;
+    set_bit128 f 
+
+inline_for_extraction
+val poly1305_encode_last: #s:field_spec -> f:felem s -> b:bytes -> 
+			len:size_t{size_v len == length b /\ length b < 16} -> Stack unit
+                   (requires (fun h -> live h b /\ live h f ))
+		   (ensures (fun h0 _ h1 -> modifies (loc_buffer f) h0 h1))
+#reset-options "--z3rlimit 100"
+let poly1305_encode_last #s f b len = 
+    push_frame();
+    let tmp = create 0uy (size 16) in
+    blit b (size 0) tmp (size 0) len;
+    let (lo,hi) = load64x2_le tmp in
+    load_felem f lo hi;
+    set_bit f (len *. size 8);
+    admit();
+    pop_frame()
+
+inline_for_extraction
+val poly1305_encode_r: #s:field_spec -> f:felem s -> b:lbytes 16 -> Stack unit
+                   (requires (fun h -> live h b /\ live h f ))
+		   (ensures (fun h0 _ h1 -> modifies (loc_buffer f) h0 h1))
+let poly1305_encode_r #s f b = 
+    let (lo,hi) = load64x2_le b in
+    let mask0 = u64 0x0ffffffc0fffffff in
+    let mask1 = u64 0x0ffffffc0ffffffc in
+    let lo = lo &. mask0 in
+    let hi = hi &. mask1 in
+    load_felem f lo hi
+  
+
+type poly1305_ctx (s:field_spec) = lbuffer (limb s) (nlimb s `op_Multiply` 4)
+
+(*
+inline_for_extraction
+val get_acc: #s:field_spec -> ctx:poly1305_ctx s -> Stack (felem s)
+                   (requires (fun h -> live h ctx))
+		   (ensures (fun h0 r h1 -> h0 == h1 /\ live h1 r))
+*)
+inline_for_extraction 
+let get_acc #s (ctx:poly1305_ctx s) = sub ctx (size 0) (size (nlimb s))
+
+
+(*
+inline_for_extraction
+val get_r: #s:field_spec -> ctx:poly1305_ctx s -> Stack (felem s)
+                   (requires (fun h -> live h ctx))
+		   (ensures (fun h0 r h1 -> h0 == h1 /\ live h1 r))
+*)
+inline_for_extraction
+let get_r #s (ctx:poly1305_ctx s) = sub ctx (size (nlimb s)) (size (nlimb s))
+
+(*
+inline_for_extraction
+val get_r_20: #s:field_spec -> ctx:poly1305_ctx s -> Stack (felem s)
+                   (requires (fun h -> live h ctx))
+		   (ensures (fun h0 r h1 -> h0 == h1 /\ live h1 r))
+*)
+inline_for_extraction
+let get_r_20 #s (ctx:poly1305_ctx s) = sub ctx (size (nlimb s) *. size 2) (size (nlimb s))
+
+(*
+inline_for_extraction
+val get_s: #s:field_spec -> ctx:poly1305_ctx s -> Stack (felem s)
+                   (requires (fun h -> live h ctx))
+		   (ensures (fun h0 r h1 -> h0 == h1 /\ live h1 r))
+*)
+inline_for_extraction
+let get_s #s (ctx:poly1305_ctx s) = sub ctx (size (nlimb s) *. size 3) (size (nlimb s))
+
+
+inline_for_extraction
+val poly1305_init: #s:field_spec -> ctx:poly1305_ctx s -> key:lbytes 32 -> Stack unit
+                   (requires (fun h -> live h ctx /\ live h key))
+		   (ensures (fun h0 _ h1 -> modifies (loc_buffer ctx) h0 h1))
+let poly1305_init #s ctx key = 
+  let kr = sub key (size 0) (size 16) in
+  let ks = sub key (size 16) (size 16) in
+  
+  let acc = get_acc ctx in
+  let r = get_r ctx in
+  let r_20 = get_r_20 ctx in
+  let sk = get_s ctx in 
+  set_zero acc;
+  poly1305_encode_r r kr;
+  smul20_felem r_20 r;
+  let (sl,sh) = load64x2_le ks in
+  load_felem sk sl sh;
+  admit()
+
+inline_for_extraction
+val poly1305_update: #s:field_spec -> ctx:poly1305_ctx s -> text:bytes -> len:size_t{size_v len == length text} -> Stack unit
+                   (requires (fun h -> live h ctx /\ live h text))
+		   (ensures (fun h0 _ h1 -> modifies (loc_buffer ctx) h0 h1))
+
+let poly1305_update #s ctx text len = 
+  push_frame();
+  let acc = sub ctx (size 0) (size 3) in
+  let r = sub ctx (size 3) (size 3) in
+  let r_20 = sub ctx (size 6) (size 3) in
+  let e = create_felem s in
+  let blocks = len /. size 16 in
+  let h0 = ST.get() in
+  admit();
+  loop_nospec #h0 blocks ctx 
+    (fun i ->
+       let b = sub text (i *. size 16) (size 16) in
+       poly1305_encode_block e b;
+       fadd_mul_felem acc e r r_20);
+  let rem = len %. size 16 in
+  if (rem >. size 0) then (
+     let b = sub text (blocks *. size 16) (size 16) in
+     poly1305_encode_last e b rem;
+     fadd_mul_felem acc e r r_20);
+  pop_frame()
+
+inline_for_extraction
+val poly1305_finish: #s:field_spec -> ctx:poly1305_ctx s -> tag:lbytes 16 -> Stack unit 
+		     (requires (fun h -> live h ctx /\ live h tag))
+		     (ensures (fun h0 _ h1 -> modifies (loc_buffer tag) h0 h1))
+		  
+let poly1305_finish #s ctx tag = 
+  let acc = get_acc ctx in
+  let sk = get_s ctx in
+  carry_felem acc;
+  carry_top_felem acc;
+  add_felem acc sk;
+  carry_felem acc;
+  let (lo,hi) = store_felem acc in
+  store64x2_le tag lo hi;
+  admit()
+
+
+inline_for_extraction
+val poly1305_mac: #s:field_spec -> tag:lbytes 16 -> text:bytes -> len:size_t{size_v len == length text} -> key:lbytes 32 -> Stack unit 
+		     (requires (fun h -> live h text /\ live h tag /\ live h key))
+ 		     (ensures (fun h0 _ h1 -> modifies (loc_buffer tag) h0 h1))
+let poly1305_mac #s tag text len key = 
+  push_frame();
+  let ctx : lbuffer (limb s) (nlimb s `op_Multiply` 4) = create (limb_zero s) (size (nlimb s) *. size 4) in
+  poly1305_init ctx key;
+  poly1305_update ctx text len;
+  poly1305_finish ctx tag;
+  pop_frame()
