code/aes/Hacl.Poly1305_64.fst
@@ -1,0 +1,5 @@
+module Hacl.Poly1305_64
+open Hacl.Impl.Poly1305.Fields
+open Lib.IntTypes
+
+let poly1305_mac o t l k = Hacl.Impl.Poly1305.poly1305_mac #M64 o t l k
