lib/Lib.IntTypes.fsti
@@ -403,7 +403,6 @@ let (=.) #t = eq #t
 
 inline_for_extraction
 let (<.) #t = lt #t
-
 inline_for_extraction
 let (<=.) #t = le #t
 
